ConNF/Counting/CodingFunctionEquiv.lean
@@ -19,19 +19,19 @@ namespace CodingFunction
 
 /-- A reordering `r` is an equivalence of coding functions if it is an equivalence of some ordered
 supports in the domains of the coding functions in question. -/
-def IsEquiv (r : Tree Reorder β) (χ₁ χ₂ : CodingFunction β) : Prop :=
-  ∃ S₁ ∈ χ₁, ∃ S₂ ∈ χ₂, OrdSupport.IsEquiv r S₁ S₂
+def Equiv (χ₁ χ₂ : CodingFunction β) : Prop :=
+  ∃ S₁ ∈ χ₁, ∃ S₂ ∈ χ₂, S₁ ≈ S₂
 
 /-- If two coding functions are equivalent, every ordered support in the domain of the first one
 is equivalent to some ordered support in the domain of the second. -/
-def exists_mem_isEquiv {r : Tree Reorder β} {χ₁ χ₂ : CodingFunction β} (h : IsEquiv r χ₁ χ₂)
+def exists_mem_equiv {χ₁ χ₂ : CodingFunction β} (h : Equiv χ₁ χ₂)
     (S₁ : OrdSupport β) (hS₁ : S₁ ∈ χ₁) :
-    ∃ S₂ ∈ χ₂, OrdSupport.IsEquiv r S₁ S₂ := by
+    ∃ S₂ ∈ χ₂, S₁ ≈ S₂ := by
   obtain ⟨T₁, hT₁, T₂, hT₂, h⟩ := h
   obtain ⟨ρ, rfl⟩ := (χ₁.dom_iff T₁ S₁ hT₁).mp hS₁
   refine ⟨ρ • T₂, ?_, ?_⟩
   · exact χ₂.smul_mem ρ hT₂
-  · exact OrdSupport.isEquiv_smul h ρ
+  · exact OrdSupport.smul_equiv_smul h ρ
 
 end CodingFunction
 
